qed ClientHist WPs for Put, SelfMon, Get. note that Get advances client next_epoch, but not hist epoch valid, so need to split those up

src/program_proof/pav/client_hist.v
@@ -10,22 +10,28 @@ Record t :=
   mk {
     γ: gname;
     uid: w64;
-    (* pks is the only difference from normal client struct. *)
+    (* pks differs from the client struct.
+    it tracks all our actual keys. *)
     pks: list map_val_ty;
-    ep_valid: w64;
+    next_epoch: w64;
+    (* hist_epoch differs from the client struct.
+    it's epoch validity for the history, which only gets updated by
+    Put and SelfMon, not Get. *)
+    hist_epoch: w64;
     serv: Server.t;
     serv_is_good: bool;
   }.
 Global Instance eta : Settable _ :=
-  settable! mk <γ; uid; pks; ep_valid; serv; serv_is_good>.
+  settable! mk <γ; uid; pks; next_epoch; hist_epoch; serv; serv_is_good>.
 
 Section defs.
 Context `{!heapGS Σ, !pavG Σ}.
 
 Definition own (ptr : loc) (obj : t) : iProp Σ :=
+  "%Hlt_ep" ∷ ⌜ uint.Z obj.(hist_epoch) <= uint.Z obj.(next_epoch) ⌝ ∗
   "Hcli" ∷ Client.own ptr (Client.mk obj.(γ) obj.(uid) (W64 $ length obj.(pks))
-    obj.(ep_valid) obj.(serv) obj.(serv_is_good)) ∗
-  "#Hhist" ∷ is_hist obj.(γ) obj.(serv).(Server.vrf_pk) obj.(uid) obj.(pks) obj.(ep_valid).
+    obj.(next_epoch) obj.(serv) obj.(serv_is_good)) ∗
+  "#Hhist" ∷ is_hist obj.(γ) obj.(serv).(Server.vrf_pk) obj.(uid) obj.(pks) obj.(hist_epoch).
 
 End defs.
 End ClientHist.
@@ -33,7 +39,7 @@ End ClientHist.
 Section proof.
 Context `{!heapGS Σ, !pavG Σ}.
 
-Lemma wp_Client__Put ptr_c c sl_pk d0 (pk : list w8) :
+Lemma wp_ClientHist__Put ptr_c c sl_pk d0 (pk : list w8) :
   {{{
     "Hcli" ∷ ClientHist.own ptr_c c ∗
     "Hsl_pk" ∷ own_slice_small sl_pk byteT d0 pk
@@ -41,8 +47,6 @@ Lemma wp_Client__Put ptr_c c sl_pk d0 (pk : list w8) :
   Client__Put #ptr_c (slice_val sl_pk)
   {{{
     err (ep : w64) ptr_err, RET (#ep, #ptr_err);
-    let new_c := set ClientHist.pks (λ x, (x ++ [(ep, pk)]))
-      (set ClientHist.ep_valid (λ _, word.add ep (W64 1)) c) in
     "Hsl_pk" ∷ own_slice_small sl_pk byteT d0 pk ∗
     "Hown_err" ∷ ClientErr.own ptr_err err c.(ClientHist.serv).(Server.sig_pk) ∗
     "%Hgenie" ∷ ⌜ c.(ClientHist.serv_is_good) = true → err.(ClientErr.Err) = false ⌝ ∗
@@ -50,31 +54,82 @@ Lemma wp_Client__Put ptr_c c sl_pk d0 (pk : list w8) :
       then
         "Hcli" ∷ ClientHist.own ptr_c c
       else
+        let new_c := set ClientHist.pks (λ x, (x ++ [(ep, pk)]))
+          (set ClientHist.next_epoch (λ _, word.add ep (W64 1))
+          (set ClientHist.hist_epoch (λ _, word.add ep (W64 1)) c)) in
         "Hcli" ∷ ClientHist.own ptr_c new_c)
   }}}.
 Proof.
   iIntros (Φ) "H HΦ". iNamed "H". iNamed "Hcli".
   destruct c. simpl in *.
-  destruct serv_is_good eqn:Heq_good.
-  - wp_apply (wp_Client__Put_good with "[$Hcli $Hsl_pk //]").
-   iIntros "*". iNamed 1. simpl in *.
-    iApply "HΦ". iFrame. iSplit; [done|].
-    rewrite Heq_err. iSplit; simpl in *.
-    { rewrite length_app. simpl.
-      replace (W64 (_ + _)%nat) with
-        (word.add (W64 $ length pks) (W64 1)); [|word].
-      iFrame. }
-    iApply (hist_extend_put with "[$Hhist $His_put_post]"); word.
-  - wp_apply (wp_Client__Put with "[$Hcli $Hsl_pk //]").
-    iIntros "*". iNamed 1. simpl in *.
-    iApply "HΦ". iFrame. iSplit; [done|].
-    case_match; [iFrame "∗#"|]. iNamed "Herr".
-    iSplit; simpl in *.
-    { rewrite length_app. simpl.
-      replace (W64 (_ + _)%nat) with
-        (word.add (W64 $ length pks) (W64 1)); [|word].
-      iFrame. }
-    iApply (hist_extend_put with "[$Hhist $His_put_post]"); word.
+  wp_apply (wp_Client__Put with "[$Hcli $Hsl_pk]").
+  simpl. iIntros "*". iNamed 1.
+  iApply "HΦ". iFrame "∗%".
+  case_match; iNamed "Herr"; [by iFrame "∗#"|].
+  iSplit; simpl in *; [done|]; iSplit.
+  - rewrite length_app. simpl.
+    replace (W64 (_ + _)%nat) with
+      (word.add (W64 $ length pks) (W64 1)); [|word].
+    iFrame.
+  - iApply hist_extend_put; [..|iFrame "#"]; try word.
+Qed.
+
+Lemma wp_ClientHist__SelfMon ptr_c c :
+  {{{
+    "Hcli" ∷ ClientHist.own ptr_c c
+  }}}
+  Client__SelfMon #ptr_c
+  {{{
+    err (ep : w64) ptr_err, RET (#ep, #ptr_err);
+    "Hown_err" ∷ ClientErr.own ptr_err err c.(ClientHist.serv).(Server.sig_pk) ∗
+    "%Hgenie" ∷ ⌜ c.(ClientHist.serv_is_good) = true → err.(ClientErr.Err) = false ⌝ ∗
+
+    "Herr" ∷ (if err.(ClientErr.Err)
+      then
+        "Hcli" ∷ ClientHist.own ptr_c c
+      else
+        let new_c := set ClientHist.next_epoch (λ _, word.add ep (W64 1))
+          (set ClientHist.hist_epoch (λ _, word.add ep (W64 1)) c) in
+        "Hcli" ∷ ClientHist.own ptr_c new_c)
+  }}}.
+Proof.
+  iIntros (Φ) "H HΦ". iNamed "H". iNamed "Hcli".
+  destruct c. simpl in *.
+  wp_apply (wp_Client__SelfMon with "[$Hcli]").
+  simpl. iIntros "*". iNamed 1.
+  iApply "HΦ". iFrame "∗%".
+  case_match; iNamed "Herr"; iFrame "∗#"; simpl; [done|].
+  iSplit; [done|].
+  (* TODO: maybe iApply bug. this doesn't work.
+  iApply (hist_extend_selfmon with "[# $]"). *)
+  iApply hist_extend_selfmon; [..|iFrame "#"]; word.
+Qed.
+
+Lemma wp_ClientHist__Get ptr_c c (uid : w64) :
+  {{{
+    "Hcli" ∷ ClientHist.own ptr_c c
+  }}}
+  Client__Get #ptr_c #uid
+  {{{
+    err sl_pk (is_reg : bool) (ep : w64) ptr_err,
+    RET (#is_reg, slice_val sl_pk, #ep, #ptr_err);
+    "Hown_err" ∷ ClientErr.own ptr_err err c.(ClientHist.serv).(Server.sig_pk) ∗
+    "%Hgenie" ∷ ⌜ c.(ClientHist.serv_is_good) = true → err.(ClientErr.Err) = false ⌝ ∗
+
+    "Herr" ∷ (if err.(ClientErr.Err)
+      then
+        "Hcli" ∷ ClientHist.own ptr_c c
+      else
+        let new_c := set ClientHist.next_epoch (λ _, word.add ep (W64 1)) c in
+        "Hcli" ∷ ClientHist.own ptr_c new_c)
+  }}}.
+Proof.
+  iIntros (Φ) "H HΦ". iNamed "H". iNamed "Hcli".
+  destruct c. simpl in *.
+  wp_apply (wp_Client__Get with "[$Hcli]").
+  simpl. iIntros "*". iNamed 1.
+  iApply "HΦ". iFrame "∗%".
+  case_match; iNamed "Herr"; iFrame "∗#"; simpl; [done|word].
 Qed.
 
 (* written in this structure to elicit the pure gs_hist,
@@ -174,10 +229,10 @@ Proof.
 Qed.
 
 Lemma logical_audit_get_msv (ep : w64) ptr_c c γaudit :
-  uint.Z ep < uint.Z c.(ClientHist.ep_valid) →
+  uint.Z ep < uint.Z c.(ClientHist.next_epoch) →
   ClientHist.own ptr_c c -∗
   logical_audit_post c.(ClientHist.γ) γaudit
-    c.(ClientHist.serv).(Server.vrf_pk) c.(ClientHist.ep_valid) -∗
+    c.(ClientHist.serv).(Server.vrf_pk) c.(ClientHist.next_epoch) -∗
   msv γaudit c.(ClientHist.serv).(Server.vrf_pk)
     ep c.(ClientHist.uid) (get_lat c.(ClientHist.pks) ep).
 Proof.
